src/Analysis/Generic/Solver/Exec/Exec_Bridge.thy
@@ -1,5 +1,5 @@
 theory Exec_Bridge
-  imports Exec_St TD_Side_Eff_Bounds TD_Side_RHS_Generator Constraint_System
+  imports Exec_Backward TD_Side_Eff_Bounds TD_Side_RHS_Generator Constraint_System
 begin
 
 section \<open>Executable equation-system refinement\<close>
